heap_model.v
@@ -37,89 +37,46 @@ Definition stack := table var adr.
 Definition heap := table adr adr.
 Definition state := (stack * heap)%type.
 
-Definition world := ((var -> option adr)*(adr -> option adr))%type.
+Definition world := ((var -> option adr)*(fpm adr adr))%type.
 
 Instance Join_world: Join world :=
   Join_prod
     (var -> option adr) (Join_equiv _)
-    (adr -> option adr) (Join_fun adr (option adr) (Join_lower (Join_discrete adr))).
+    (fpm adr adr) (Join_fpm (Join_discrete adr)).
 
-Instance Perm_world : Perm_alg world := _.
-Instance Sep_world : Sep_alg world := _.
+Instance Perm_world : Perm_alg world.
+apply Perm_prod; [apply Perm_equiv | apply Perm_fpm; apply Perm_discrete].
+Qed.
+
+Instance Sep_world : Sep_alg world.
+apply Sep_prod. apply Sep_equiv. apply Sep_fpm.
+Qed.
 
 Instance Canc_world : Canc_alg world.
-apply Canc_prod; [apply Canc_equiv | apply Canc_fun, Canc_lower; [intuition | repeat intro; inversion H]].
+apply Canc_prod; [apply Canc_equiv | apply Canc_fpm; [intuition | repeat intro; inversion H]].
 Qed.
 
 Instance Disj_world : Disj_alg world.
-apply Disj_prod; [apply Disj_equiv | apply Disj_fun, Disj_lower; repeat intro; inversion H].
-Qed.
-
-Instance Cross_opt_adr : @Cross_alg (option adr) (@Join_lower adr (Join_discrete adr)).
-repeat intro.
-assert (X : @Cross_alg adr (Join_discrete adr)) by (repeat intro; inv H1).
-icase a; icase b; icase z; icase c; icase d;
-let Heq := fresh "Heq" in
-repeat match goal with
-         | [H : join (Some _) (Some _) None |- _] => exfalso; inv H
-         | [H : join (Some _) None None |- _] => exfalso; inv H
-         | [H : join None None (Some _) |- _] => exfalso; inv H
-         | [H : join None (Some _) None |- _] => exfalso; inv H
-         | [H : join (Some ?Xa) (Some ?Ya) (Some ?Za) |- _] => assert (join Xa Ya Za) by (inv H; trivial); clear H
-         | [H : join (Some ?Xa) None (Some ?Ya) |- _] =>
-           assert (Heq: Xa = Ya) by (inv H; trivial); clear H; rewrite Heq in *; clear Heq Xa
-         | [H : join None (Some ?Xa) (Some ?Ya) |- _] =>
-           assert (Heq: Xa = Ya) by (inv H; trivial); clear H; rewrite Heq in *; clear Heq Xa
-       end.
-Ltac solve_lower :=
-  repeat split;
-  match goal with
-    | [|- join (Some ?Xa) None (Some ?Xa)] => apply lower_None2
-    | [|- join None (Some ?Xa) (Some ?Xa)] => apply lower_None1
-    | [|- join None None None] => apply lower_None1
-    | [H: join ?Xa ?Ya ?Za |- join (Some ?Xa) (Some ?Ya) (Some ?Za)] => apply lower_Some; apply H
-  end.
-destruct (X a a0 a2 a3 a1 H0 H1) as [[[[ac ad] bc] bd] [? [? [? ?]]]];
-  exists (Some ac, Some ad, Some bc, Some bd); solve_lower.
-exists (Some a, None, Some a0, None); solve_lower.
-exists (None, Some a, None, Some a0); solve_lower.
-exists (Some a1, Some a2, None, None); solve_lower.
-exists (Some a0, None, None, None); solve_lower.
-exists (None, Some a0, None, None); solve_lower.
-exists (None, None, Some a1, Some a2); solve_lower.
-exists (None, None, Some a0, None); solve_lower.
-exists (None, None, None, Some a0); solve_lower.
-exists (None, None, None, None); solve_lower.
+apply Disj_prod; [apply Disj_equiv | apply Disj_fpm; repeat intro; inversion H].
 Qed.
 
 Instance Cross_world : Cross_alg world.
-apply Cross_prod.
-apply Cross_equiv.
-repeat intro.
-pose (f (x: adr) := projT1 (Cross_opt_adr (a x) (b x) (c x) (d x) (z x) (H x) (H0 x))).
-pose (g (x: adr) := projT2 (Cross_opt_adr (a x) (b x) (c x) (d x) (z x) (H x) (H0 x))).
-pose (ac (x: adr) := fst (fst (fst (f x)))).
-pose (ad (x: adr) := snd (fst (fst (f x)))).
-pose (bc (x: adr) := snd (fst (f x))).
-pose (bd (x: adr) := snd (f x)).
-exists (ac,ad,bc,bd); unfold ac, ad, bc, bd, f; clear ac ad bc bd f.
-repeat split; intro x; simpl; generalize (g x);
-destruct (projT1 (Cross_opt_adr (a x) (b x) (c x) (d x) (z x) (H x) (H0 x))) as [[[? ?] ?] ?]; simpl; intuition.
+apply Cross_prod; [apply Cross_equiv | apply Cross_fpm; [apply Perm_discrete | apply psa_discrete | repeat intro; inv H]].
 Qed.
 
 Definition fun_set (f: nat -> option nat) (x: nat) (y: option nat) :=
   fun i => if eq_dec i x then y else f i.
 
 Definition subst (x y: var) (P: pred world) : pred world :=
-  fun w => P (fun_set (fst w) x (fst w y), snd w). 
+  fun w => P (fun_set (fst w) x (fst w y), snd w).
 
 Definition mapsto (x y: var) : pred world :=
   fun w => x <> 0 /\
     exists ax, fst w x = Some ax /\
                exists ay, fst w y = Some ay /\
-                          (forall a, a <> ax -> snd w a = None) /\ snd w ax = Some ay.
+                          (forall a, a <> ax -> lookup_fpm (snd w) a = None) /\ lookup_fpm (snd w) ax = Some ay.
 
-Lemma precise_mapsto: forall x y, precise(mapsto x y).
+Lemma precise_mapsto: forall x y, precise (mapsto x y).
 Proof.
   repeat intro; destruct w1 as [r1 m1]; destruct w2 as [r2 m2]; destruct w as [r m].
   destruct H1 as [[rx mx] [[? ?] ?]]; destruct H2 as [[ry my] [[? ?] ?]]; simpl in H1, H2, H3, H4, H5, H6.
@@ -128,10 +85,11 @@ Proof.
   destruct H0 as [? [ax2 [? [ay2 [? [? ?]]]]]]; simpl in H8, H9, H10, H11.
   rewrite H7 in *; clear H7 r1. rewrite H1 in H8; inversion H8. rewrite H12 in *; clear H12 ax1.
   rewrite H2 in H9; inversion H9; rewrite H12 in *; clear H12 ay1.
-  assert (m1 = m2). extensionality mm; destruct (eq_dec mm ax2).
-  rewrite e in *; rewrite H5, H11; trivial.
+  destruct m1 as [x1 f1]; destruct m2 as [x2 f2]; simpl in *.
+  f_equal; trivial. apply exist_ext.
+  extensionality mm; destruct (eq_dec mm ax2).
+  rewrite e in *. rewrite H5, H11; trivial.
   specialize(H3 mm n); specialize (H10 mm n); rewrite H3, H10; trivial.
-  repeat f_equal; trivial.
 Qed.
 
 Definition equal (x y: var) : pred world := fun w => fst w x = fst w y.
